@prefix : <http://curiocity.org/> .
@prefix owl: <http://www.w3.org/2002/07/owl#> .
@prefix rdf: <http://www.w3.org/1999/02/22-rdf-syntax-ns#> .
@prefix xml: <http://www.w3.org/XML/1998/namespace> .
@prefix xsd: <http://www.w3.org/2001/XMLSchema#> .
@prefix rdfs: <http://www.w3.org/2000/01/rdf-schema#> .
@base <http://curiocity.org/> .

<http://curiocity.org/> rdf:type owl:Ontology ;
                         rdfs:comment """CURIOCITY Cultural Heritage in Urban Tourism

Ranking add-on for CURIOCITY."""@en ;
                         rdfs:label "CURIOCITY-RANKING"@en .

#################################################################
#    Object Properties
#################################################################

###  http://curiocity.org/is_ranked_by
:is_ranked_by rdf:type owl:ObjectProperty .


###  http://curiocity.org/ranks
:ranks rdf:type owl:ObjectProperty .


#################################################################
#    Data properties
#################################################################

###  http://curiocity.org/has_rank_value
:has_rank_value rdf:type owl:DatatypeProperty ;
                rdfs:domain <http://curiocity.org/#Rank_Assignment> ;
                rdfs:range rdfs:Literal ;
                rdfs:comment "Rank value. Need to change to correspondent literal according to qualification range."@en ;
                rdfs:label "has rank value"@en .


#################################################################
#    Classes
#################################################################

###  http://curiocity.org/Profile
:Profile rdf:type owl:Class ;
         rdfs:subClassOf <http://erlangen-crm.org/170309/E39_Actor> ;
         rdfs:comment """Scope note:
This class comprises real persons who live or are assumed to have lived and they are not historical figures. This class describes people with the purpose of using their data in social or ranking activities. Compare with crm:E21 Person 

This class describes a participant of a ranking event. Point of extension to ontologies related to people domain. (e.g. FOAF - foaf:agent)"""@en ;
         rdfs:label "Profile"@en .


###  http://curiocity.org/#Rank_Assignment
<http://curiocity.org/#Rank_Assignment> rdf:type owl:Class ;
                                        rdfs:subClassOf <http://erlangen-crm.org/170309/E13_Attribute_Assignment> ;
                                        rdfs:comment "This class describes events where an Exhibit is evaluated or score assigned by a Profile."@en ;
                                        rdfs:label "Rank Assignment"@en .


###  http://erlangen-crm.org/170309/E13_Attribute_Assignment
<http://erlangen-crm.org/170309/E13_Attribute_Assignment> rdf:type owl:Class ;
                                                          rdfs:label "E13 Attribute Assignment"@en .


###  http://erlangen-crm.org/170309/E39_Actor
<http://erlangen-crm.org/170309/E39_Actor> rdf:type owl:Class ;
                                           rdfs:label "E39 Actor"@en .


###  Generated by the OWL API (version 4.5.9.2019-02-01T07:24:44Z) https://github.com/owlcs/owlapi
